Stronger completeness proof for the executable semantics.
The proof now uses the stronger notion of memory permutation instead of a more
general memory refinement. We have also proven that memory permutations are
symmetric.

refinements.v
@@ -245,30 +245,144 @@ Ltac refine_inversion_all :=
      first [is_var X; is_var Y; fail 1|refine_inversion H]
   end.
 
+Record memenv_refine' `{Env Ti} (Γ : env Ti)
+    (α : bool) (f : meminj Ti) (Γm1 Γm2 : memenv Ti) := {
+  memenv_refine_injective' : meminj_injective f;
+  memenv_refine_typed_l o1 o2 r τ1 :
+    f !! o1 = Some (o2,r) → Γm1 ⊢ o1 : τ1 →
+    ∃ τ2, Γm2 ⊢ o2 : τ2 ∧ Γ ⊢ r : τ2 ↣ τ1;
+  memenv_refine_typed_r o1 o2 r τ2 :
+    f !! o1 = Some (o2,r) → Γm2 ⊢ o2 : τ2 →
+    ∃ τ1, Γm1 ⊢ o1 : τ1 ∧ Γ ⊢ r : τ2 ↣ τ1;
+  memenv_refine_alive_l o1 o2 r :
+    f !! o1 = Some (o2,r) → index_alive Γm1 o1 → index_alive Γm2 o2;
+  memenv_refine_alive_r o1 o2 r :
+    ¬α → f !! o1 = Some (o2,r) → index_alive Γm2 o2 → index_alive Γm1 o1;
+  memenv_refine_perm_l' o1 τ1 :
+    ¬α → Γm1 ⊢ o1 : τ1 → ∃ o2, f !! o1 = Some (o2,[]);
+  memenv_refine_perm_r' o2 τ2 :
+    ¬α → Γm2 ⊢ o2 : τ2 → ∃ o1, f !! o1 = Some (o2,[])
+}.
+Arguments memenv_refine_typed_l {_ _ _ _ _ _ _} _ _ _ _ _ _ _.
+Arguments memenv_refine_typed_r {_ _ _ _ _ _ _} _ _ _ _ _ _ _.
+Arguments memenv_refine_alive_l {_ _ _ _ _ _ _} _ _ _ _ _ _.
+Arguments memenv_refine_alive_r {_ _ _ _ _ _ _} _ _ _ _ _ _ _.
+
 Instance memenv_refine `{Env Ti} :
-    RefineM Ti (env Ti) (memenv Ti) := λ Γ α f Γm1 Γm2,
-  (**i 1.) *) meminj_injective f ∧
-  (**i 2.) *) (∀ o1 o2 r τ1, f !! o1 = Some (o2,r) →
-    Γm1 ⊢ o1 : τ1 → ∃ τ2, Γm2 ⊢ o2 : τ2 ∧ Γ ⊢ r : τ2 ↣ τ1) ∧
-  (**i 3.) *) (∀ o1 o2 r τ2, f !! o1 = Some (o2,r) →
-    Γm2 ⊢ o2 : τ2 → ∃ τ1, Γm1 ⊢ o1 : τ1 ∧ Γ ⊢ r : τ2 ↣ τ1) ∧
-  (**i 4.) *) (∀ o1 o2 r, f !! o1 = Some (o2,r) →
-    index_alive Γm1 o1 → index_alive Γm2 o2) ∧
-  (**i 5.) *) (∀ o1 o2 r, ¬α → f !! o1 = Some (o2,r) → r = []).
+  RefineM Ti (env Ti) (memenv Ti) := memenv_refine'.
+
 Record meminj_extend {Ti} (f f' : meminj Ti) (Γm1 Γm2 : memenv Ti) := {
   meminj_extend_left o τ : Γm1 ⊢ o : τ → f' !! o = f !! o;
   meminj_extend_right o o' r τ :
     Γm2 ⊢ o' : τ → f' !! o = Some (o',r) → f !! o = Some (o',r)
 }.
 
+Definition meminj_inverse {Ti} (f : meminj Ti) : meminj Ti :=
+  match f with
+  | meminj_id => meminj_id
+  | meminj_map f => meminj_map $ map_of_list $ (λ o1o2r,
+      let '(o1,(o2,_)) := o1o2r in (o2,(o1,[]))) <$> map_to_list f
+  end.
+
 Section memenv_refine.
 Context `{EnvSpec Ti}.
 Implicit Types α : bool.
 Implicit Types f : meminj Ti.
+Local Arguments lookup _ _ _ _ _ !_ /.
 
 Lemma memenv_refine_injective Γ α f Γm1 Γm2 :
   Γm1 ⊑{Γ,α,f} Γm2 → meminj_injective f.
 Proof. by intros [??]. Qed.
+Lemma memenv_refine_perm_l Γ f Γm1 Γm2 o1 τ :
+  Γm1 ⊑{Γ,false,f} Γm2 → Γm1 ⊢ o1 : τ →
+  ∃ o2, f !! o1 = Some (o2,[]) ∧ Γm2 ⊢ o2 : τ.
+Proof.
+  intros [_ Hl _ _ _ Hl' _] ?. destruct (Hl' o1 τ) as [o2 ?]; auto.
+  destruct (Hl o1 o2 [] τ) as (?&?&?); simplify_type_equality; eauto.
+Qed.
+Lemma memenv_refine_perm_r Γ f Γm1 Γm2 o2 τ :
+  Γm1 ⊑{Γ,false,f} Γm2 → Γm2 ⊢ o2 : τ →
+  ∃ o1, f !! o1 = Some (o2,[]) ∧ Γm1 ⊢ o1 : τ.
+Proof.
+  intros [_ _ Hr _ _ _ Hr'] ?. destruct (Hr' o2 τ) as [o1 ?]; auto.
+  destruct (Hr o1 o2 [] τ) as (τ2&?&?); simplify_type_equality; eauto.
+Qed.
+Lemma lookup_meminj_inverse_1_help Γ f Γm1 Γm2 o1 o2 r1 :
+  Γm1 ⊑{Γ,false,f} Γm2 → meminj_inverse f !! o2 = Some (o1,r1) →
+  ∃ r2, f !! o1 = Some (o2,r2) ∧ r1 = [].
+Proof.
+  destruct f as [|f]; simpl; intros HΓm Ho2; [naive_solver|].
+  apply elem_of_map_of_list_2 in Ho2; revert Ho2.
+  rewrite elem_of_list_fmap; intros ((o1'&o2'&r2')&?&Ho1'); simplify_equality'.
+  apply elem_of_map_to_list in Ho1'; eauto.
+Qed.
+Lemma lookup_meminj_inverse_1 Γ f Γm1 Γm2 o1 o2 r τ :
+  Γm1 ⊑{Γ,false,f} Γm2 → meminj_inverse f !! o2 = Some (o1,r) →
+  Γm2 ⊢ o2 : τ → Γm1 ⊢ o1 : τ ∧ f !! o1 = Some (o2,[]) ∧ r = [].
+Proof.
+  intros HΓm ??.
+  destruct (lookup_meminj_inverse_1_help Γ f Γm1 Γm2 o1 o2 r) as (r'&?&?); auto.
+  destruct (memenv_refine_perm_r Γ f Γm1 Γm2 o2 τ) as (o1'&?&?); auto.
+  destruct (memenv_refine_injective Γ false f
+    Γm1 Γm2 HΓm o1 o1' o2 r' []); simplify_equality'; auto.
+  by destruct (ref_disjoint_nil_inv_l r').
+Qed.
+Lemma lookup_meminj_inverse_2 Γ f Γm1 Γm2 o1 o2 r2 τ :
+  Γm1 ⊑{Γ,false,f} Γm2 → Γm1 ⊢ o1 : τ →
+  f !! o1 = Some (o2,r2) → meminj_inverse f !! o2 = Some (o1,[]).
+Proof.
+  destruct f as [|f]; simpl; [naive_solver|]; intros HΓm ??.
+  apply elem_of_map_of_list_1_help.
+  { rewrite elem_of_list_fmap.
+    eexists (o1,(o2,r2)); split; auto. by apply elem_of_map_to_list. }
+  intros [??]; rewrite elem_of_list_fmap;
+    intros ((o1'&o2'&r2')&?&Ho1'); simplify_equality; f_equal.
+  apply elem_of_map_to_list in Ho1'.
+  destruct (memenv_refine_injective Γ false (meminj_map f)
+    Γm1 Γm2 HΓm o1 o1' o2' r2 r2'); simplify_equality'; auto.
+  destruct (memenv_refine_perm_l Γ (meminj_map f) Γm1 Γm2 o1 τ)
+    as (?&?&?); simplify_equality'; auto.
+  by destruct (ref_disjoint_nil_inv_l r2').
+Qed.
+Lemma memenv_refine_inverse Γ f Γm1 Γm2 :
+  Γm1 ⊑{Γ,false,f} Γm2 → Γm2 ⊑{Γ,false,meminj_inverse f} Γm1.
+Proof.
+  intros HΓm. constructor.
+  * intros o2 o2' o1 r1 r1' ??.
+    destruct (lookup_meminj_inverse_1_help Γ f Γm1 Γm2 o1 o2 r1); auto.
+    destruct (lookup_meminj_inverse_1_help Γ f Γm1 Γm2 o1 o2' r1');naive_solver.
+  * intros o2 o1 r τ ??.
+    destruct (lookup_meminj_inverse_1 Γ f Γm1 Γm2 o1 o2 r τ) as (?&?&->); auto.
+    eauto using ref_typed_nil_2.
+  * intros o1 o2 r τ ??.
+    destruct (lookup_meminj_inverse_1_help Γ f Γm1 Γm2 o2 o1 r) as (r'&?&->),
+      (memenv_refine_perm_l Γ f Γm1 Γm2 o2 τ) as (o2'&?&?); auto.
+    simplify_equality; eauto using ref_typed_nil_2.
+  * intros o2 o1 r ?. destruct (lookup_meminj_inverse_1_help Γ f Γm1 Γm2
+      o1 o2 r) as (?&?&?); eauto using memenv_refine_alive_r.
+  * intros o1 o2 r ??. destruct (lookup_meminj_inverse_1_help Γ f Γm1 Γm2
+      o2 o1 r) as (?&?&?); eauto using memenv_refine_alive_l.
+  * intros o2 τ2 ??. destruct (memenv_refine_perm_r Γ f Γm1 Γm2 o2 τ2)
+      as (o1&?&?); eauto using lookup_meminj_inverse_2.
+  * intros o1 τ1 ??. destruct (memenv_refine_perm_l Γ f Γm1 Γm2 o1 τ1)
+      as (o2&?&?); eauto using lookup_meminj_inverse_2.
+Qed.
+Lemma memenv_refine_inverse_compose Γ f Γm1 Γm2 o1 τ1 :
+  Γm1 ⊑{Γ,false,f} Γm2 →
+  Γm1 ⊢ o1 : τ1 → (meminj_inverse f ◎ f) !! o1 = Some (o1,[]).
+Proof.
+  intros HΓm ?; rewrite lookup_meminj_compose_Some.
+  destruct (memenv_refine_perm_l Γ f Γm1 Γm2 o1 τ1) as (o2&?&?); auto.
+  eexists o2, [], []; eauto using lookup_meminj_inverse_2.
+Qed.
+Lemma memenv_refine_compose_inverse Γ f Γm1 Γm2 o2 τ2 :
+  Γm1 ⊑{Γ,false,f} Γm2 →
+  Γm2 ⊢ o2 : τ2 → (f ◎ meminj_inverse f) !! o2 = Some (o2,[]).
+Proof.
+  intros HΓm ?; rewrite lookup_meminj_compose_Some.
+  destruct (memenv_refine_perm_r Γ f Γm1 Γm2 o2 τ2) as (o1&?&?); auto.
+  eexists o1, [], []; eauto using lookup_meminj_inverse_2.
+Qed.
 Lemma memenv_refine_id Γ Γm α : Γm ⊑{Γ,α} Γm.
 Proof.
   repeat split; intros until 0; rewrite ?lookup_meminj_id;
@@ -278,21 +392,34 @@ Lemma memenv_refine_compose Γ α1 α2 f1 f2 Γm1 Γm2 Γm3 :
   ✓ Γ → Γm1 ⊑{Γ,α1,f1} Γm2 → Γm2 ⊑{Γ,α2,f2} Γm3 →
   Γm1 ⊑{Γ,α1||α2,f2 ◎ f1} Γm3.
 Proof.
-  intros ? (?&?&?&?) (?&?&?&?);
-    repeat split; eauto using meminj_compose_injective.
-  * intros o1 o3 r τ1; rewrite lookup_meminj_compose_Some;
-      intros (o2&r2&r3&?&?&->) ?; setoid_rewrite ref_typed_app; naive_solver.
-  * intros o1 o3 r τ2; rewrite lookup_meminj_compose_Some;
-      intros (o2&r2&r3&?&?&->) ?; setoid_rewrite ref_typed_app; naive_solver.
-  * intros o1 o3 r; rewrite lookup_meminj_compose_Some; naive_solver.
-  * intros o1 o3 r; rewrite lookup_meminj_compose_Some; naive_solver.
+  intros ? HΓm12 HΓm23; repeat split.
+  * eauto using meminj_compose_injective, memenv_refine_injective.
+  * intros o1 o3 r τ1; rewrite lookup_meminj_compose_Some.
+    intros (o2&r2&r3&?&?&->) ?; setoid_rewrite ref_typed_app.
+    destruct (memenv_refine_typed_l HΓm12 o1 o2 r2 τ1) as (τ2&?&?); auto.
+    destruct (memenv_refine_typed_l HΓm23 o2 o3 r3 τ2) as (τ3&?&?); eauto.
+  * intros o1 o3 r τ3; rewrite lookup_meminj_compose_Some.
+    intros (o2&r2&r3&?&?&->) ?; setoid_rewrite ref_typed_app.
+    destruct (memenv_refine_typed_r HΓm23 o2 o3 r3 τ3) as (τ2&?&?); auto.
+    destruct (memenv_refine_typed_r HΓm12 o1 o2 r2 τ2) as (τ1&?&?); eauto.
+  * intros o1 o3 r; rewrite lookup_meminj_compose_Some.
+    intros (o2&r2&r3&?&?&->) ?. do 2 (eapply memenv_refine_alive_l; eauto).
+  * intros o1 o3 r ?; rewrite lookup_meminj_compose_Some.
+    intros (o2&r2&r3&?&?&->) ?. do 2 (eapply memenv_refine_alive_r; eauto).
+  * intros o1 τ1 ??; setoid_rewrite lookup_meminj_compose_Some.
+    destruct α1, α2; simplify_equality'; try done.
+    destruct (memenv_refine_perm_l Γ f1 Γm1 Γm2 o1 τ1) as (o2&?&?); auto.
+    destruct (memenv_refine_perm_l Γ f2 Γm2 Γm3 o2 τ1) as (o3&?&?); auto.
+    eexists o3, o2, [], []; eauto.
+  * intros o3 τ3 ??; setoid_rewrite lookup_meminj_compose_Some.
+    destruct α1, α2; simplify_equality'; try done.
+    destruct (memenv_refine_perm_r Γ f2 Γm2 Γm3 o3 τ3) as (o2&?&?); auto.
+    destruct (memenv_refine_perm_r Γ f1 Γm1 Γm2 o2 τ3) as (o1&?&?); auto.
+    eexists o1, o2, [], []; eauto.
 Qed.
 Lemma memenv_refine_weaken Γ Γ' α α' f Γm1 Γm2 :
   ✓ Γ → Γm1 ⊑{Γ,α,f} Γm2 → Γ ⊆ Γ' → (α → α') → Γm1 ⊑{Γ',α',f} Γm2.
-Proof.
-  intros ? (?&Htyped&Htyped'&?&?) ?; split;
-    naive_solver eauto using ref_typed_weaken.
-Qed.
+Proof. destruct 2; split; naive_solver eauto using ref_typed_weaken. Qed.
 Lemma meminj_extend_reflexive f Γm1 Γm2 : meminj_extend f f Γm1 Γm2.
 Proof. by split. Qed.
 Lemma meminj_extend_transitive f f' f'' Γm1 Γm2 Γm1' Γm2' :
@@ -311,5 +438,23 @@ Proof.
     intros (o'&r'&r''&Ho&Ho'&->). eapply Hf' in Ho'; eauto.
     rewrite lookup_meminj_id in Ho'; simplify_equality.
     rewrite (right_id_L [] (++)); eauto using memenv_forward_typed.
+Qed.
+Lemma meminj_extend_inverse Γ f1 f2 Γm1 Γm2 Γm1' Γm2' :
+  Γm1 ⊑{Γ,false,f1} Γm2 → Γm2' ⊑{Γ,false,f2} Γm1' →
+  Γm1 ⇒ₘ Γm1' → Γm2 ⇒ₘ Γm2' →
+  meminj_extend (meminj_inverse f1) f2 Γm2 Γm1 →
+  meminj_extend f1 (meminj_inverse f2) Γm1 Γm2.
+Proof.
+  intros HΓ1 HΓ2 ?? [Hf Hf']; split.
+  * intros o1 τ ?. destruct (memenv_refine_perm_l Γ f1
+      Γm1 Γm2 o1 τ) as (o2&Ho1&?); auto; rewrite Ho1.
+    eapply lookup_meminj_inverse_2; eauto using memenv_forward_typed.
+    erewrite Hf by eauto; eauto using lookup_meminj_inverse_2.
+  * intros o1 o2 r τ ??.
+    destruct (memenv_refine_perm_r Γ f1 Γm1 Γm2 o2 τ) as (o1'&?&?); auto.
+    destruct (lookup_meminj_inverse_1_help Γ f2 Γm2' Γm1' o2 o1 r)
+      as (r'&Ho1&->); auto; erewrite Hf in Ho1 by eauto.
+    destruct (lookup_meminj_inverse_1 Γ f1 Γm1 Γm2 o1 o2 r' τ)
+      as (?&?&?); auto.
 Qed.
 End memenv_refine.
